notes on tutorial

tutorial/lithium/tutorial.v
@@ -4,54 +4,63 @@ From lithium Require Import all.
 From lithium.tutorial Require Import lang notation primitive_laws.
 Set Default Proof Using "Type".
 
-(** * Definitions and setup *)
+(** * Definitions of Lithium functions *)
+(** First, we define the Lithium functions that we will use later. *)
 Section definitions.
   Context `{!tutorialGS Σ}.
 
-  Definition check_expr (e : expr) (G : val → iProp Σ) : iProp Σ.
+  Definition expr_ok (e : expr) (G : val → iProp Σ) : iProp Σ.
   Admitted.
-  Class CheckExpr (e : expr) : Type :=
-    check_expr_proof G : iProp_to_Prop (check_expr e G).
 
-  Definition check_binop (op : bin_op) (v1 v2 : val) (G : val → iProp Σ) : iProp Σ.
+  Definition binop_ok (op : bin_op) (v1 v2 : val) (G : val → iProp Σ) : iProp Σ.
   Admitted.
-  Class CheckBinop (op : bin_op) (v1 v2 : val) : Type :=
-    check_binop_proof G : iProp_to_Prop (check_binop op v1 v2 G).
 
-  Definition check_unop (op : un_op) (v : val) (G : val → iProp Σ) : iProp Σ.
+  Definition unop_ok (op : un_op) (v : val) (G : val → iProp Σ) : iProp Σ.
   Admitted.
-  Class CheckUnop (op : un_op) (v : val) : Type :=
-    check_unop_proof G : iProp_to_Prop (check_unop op v G).
 
-  Definition check_if (v : val) (G1 G2 : iProp Σ) : iProp Σ.
+  Definition if_ok (v : val) (G1 G2 : iProp Σ) : iProp Σ.
   Admitted.
-  Class CheckIf (v : val) : Type :=
-    check_if_proof G1 G2 : iProp_to_Prop (check_if v G1 G2).
 End definitions.
+
+(** * Boilerplate for setup *)
+(** The following code is necessary to register the Lithium functions.
+You can ignore it for the purposes of this tutorial. *)
+Section setup.
+  Context `{!tutorialGS Σ}.
+
+  Class ExprOk (e : expr) : Type :=
+    expr_ok_proof G : iProp_to_Prop (expr_ok e G).
+  Class BinopOk (op : bin_op) (v1 v2 : val) : Type :=
+    binop_ok_proof G : iProp_to_Prop (binop_ok op v1 v2 G).
+  Class UnopOk (op : un_op) (v : val) : Type :=
+    unop_ok_proof G : iProp_to_Prop (unop_ok op v G).
+  Class IfOk (v : val) : Type :=
+    if_ok_proof G1 G2 : iProp_to_Prop (if_ok v G1 G2).
+End setup.
 
 Ltac generate_i2p_instance_to_tc_hook arg c ::=
   lazymatch c with
-  | check_expr ?x1 => constr:(CheckExpr x1)
-  | check_binop ?x1 ?x2 ?x3 => constr:(CheckBinop x1 x2 x3)
-  | check_unop ?x1 ?x2 => constr:(CheckUnop x1 x2)
-  | check_if ?x1 => constr:(CheckIf x1)
+  | expr_ok ?x1 => constr:(ExprOk x1)
+  | binop_ok ?x1 ?x2 ?x3 => constr:(BinopOk x1 x2 x3)
+  | unop_ok ?x1 ?x2 => constr:(UnopOk x1 x2)
+  | if_ok ?x1 => constr:(IfOk x1)
   end.
 Ltac liExtensible_to_i2p_hook P bind cont ::=
   lazymatch P with
-  | check_expr ?e ?G =>
-      cont uconstr:(((_ : CheckExpr _) _))
-  | check_binop ?op ?v1 ?v2 ?G =>
-      cont uconstr:(((_ : CheckBinop _ _ _) _))
-  | check_unop ?op ?v ?G =>
-      cont uconstr:(((_ : CheckUnop _ _) _))
-  | check_if ?v ?G1 ?G2 =>
-      cont uconstr:(((_ : CheckIf _) _ _))
+  | expr_ok ?e ?G =>
+      cont uconstr:(((_ : ExprOk _) _))
+  | binop_ok ?op ?v1 ?v2 ?G =>
+      cont uconstr:(((_ : BinopOk _ _ _) _))
+  | unop_ok ?op ?v ?G =>
+      cont uconstr:(((_ : UnopOk _ _) _))
+  | if_ok ?v ?G1 ?G2 =>
+      cont uconstr:(((_ : IfOk _) _ _))
   end.
 
 Ltac liToSyntax_hook ::=
-  change (check_expr ?x1) with (li.bind1 (check_expr x1));
-  change (check_binop ?x1 ?x2 ?x3) with (li.bind1 (check_binop x1 x2 x3));
-  change (check_unop ?x1 ?x2) with (li.bind1 (check_unop x1 x2)).
+  change (expr_ok ?x1) with (li.bind1 (expr_ok x1));
+  change (binop_ok ?x1 ?x2 ?x3) with (li.bind1 (binop_ok x1 x2 x3));
+  change (unop_ok ?x1 ?x2) with (li.bind1 (unop_ok x1 x2)).
 
 Ltac liTStep :=
  liEnsureInvariant;
@@ -61,9 +70,39 @@ Ltac liTStep :=
 
 
 (** * Tutorial *)
-
+(** This is the start of the actual tutorial. *)
 Section proofs.
   Context `{!tutorialGS Σ}.
+
+  (*
+   Open questions / comments:
+   - better name for check? verify? it is some symbolic evaluation?!
+     -> changed to _ok (which reads more like a judgement than a function name)
+   - better names for exhale and inhale? assert and assume? produce and consume?
+     Simon likes assert and assume.
+   - highlight that lithium is based on continuation passing style
+      - the monad syntax just makes this easier to read
+      - this is quite different from other approaches which do a fixed symbolic execution of the program and then mainly focus for cancellation / frame inference
+      - somewhere in the thesis, not sure where?
+   - can we get rid of the { } on the right of the bind?
+   - Youngju: interesting part is find_in_context, there it really starts to look like a custom language with primitives specifically for verification
+   - Simon: can probably immediately start with the separation logic part?
+
+   - Simon: should stick with logic programming language and call the expr_ok and friends judgements, instead of programming language and functions
+     - TODO: find out what logic programming is and how their judgements look like and what terminology they use
+     - maybe call it a logic programming language such that people are not surprised by the extensible function definitions?
+     - functions seems like a better name than judgements (or predicates from logic programming) since they have inputs and outputs
+    *)
+
+  (** Framing: Lithium is a logic programming language for building
+  automated and foundational separation logic verifiers (proof search
+  procedures?)
+
+  Key selling points:
+  - language generic
+  - automated
+  - foundational / proof producing
+ *)
 
   (** ** straight line code *)
   Definition main_code : expr :=
@@ -73,7 +112,7 @@ Section proofs.
 
   Lemma main_code_correct :
     ⊢ [{
-      _ ← {check_expr main_code};
+      _ ← {expr_ok main_code};
       done
     }].
   Proof.
@@ -81,18 +120,18 @@ Section proofs.
     repeat liTStep; liShow.
   Abort.
 
-  Lemma check_expr_Let x e1 e2 G :
-    check_expr (Let x e1 e2) G ::=
-      v1 ← {check_expr e1};
-      v2 ← {check_expr (subst' x v1 e2)};
+  Lemma expr_ok_Let x e1 e2 G :
+    expr_ok (Let x e1 e2) G :-
+      v1 ← {expr_ok e1};
+      v2 ← {expr_ok (subst' x v1 e2)};
       return G v2.
   Proof. Admitted.
-  Definition check_expr_Let_inst := [instance check_expr_Let].
-  Global Existing Instance check_expr_Let_inst | 2.
+  Definition expr_ok_Let_inst := [instance expr_ok_Let].
+  Global Existing Instance expr_ok_Let_inst | 2.
 
   Lemma main_code_correct :
     ⊢ [{
-      _ ← {check_expr main_code};
+      _ ← {expr_ok main_code};
       done
     }].
   Proof.
@@ -100,15 +139,15 @@ Section proofs.
     repeat liTStep; liShow.
   Abort.
 
-  Lemma check_expr_val v G :
-    check_expr (Val v) G ::= return G v.
+  Lemma expr_ok_val v G :
+    expr_ok (Val v) G :- return G v.
   Proof. Admitted.
-  Definition check_expr_val_inst := [instance check_expr_val].
-  Global Existing Instance check_expr_val_inst.
+  Definition expr_ok_val_inst := [instance expr_ok_val].
+  Global Existing Instance expr_ok_val_inst.
 
   Lemma main_code_correct :
     ⊢ [{
-      _ ← {check_expr main_code};
+      _ ← {expr_ok main_code};
       done
     }].
   Proof.
@@ -116,32 +155,32 @@ Section proofs.
     repeat liTStep; liShow.
   Abort.
 
-  Lemma check_expr_binop op e1 e2 G :
-    check_expr (BinOp op e1 e2) G ::=
-      v1 ← {check_expr e1};
-      v2 ← {check_expr e2};
-      v  ← {check_binop op v1 v2};
+  Lemma expr_ok_binop op e1 e2 G :
+    expr_ok (BinOp op e1 e2) G :-
+      v1 ← {expr_ok e1};
+      v2 ← {expr_ok e2};
+      v  ← {binop_ok op v1 v2};
       return G v.
   Proof. Admitted.
-  Definition check_expr_binop_inst := [instance check_expr_binop].
-  Global Existing Instance check_expr_binop_inst.
+  Definition expr_ok_binop_inst := [instance expr_ok_binop].
+  Global Existing Instance expr_ok_binop_inst.
 
-  Lemma check_binop_plus_int_int (n1 n2 : Z) G :
-    check_binop PlusOp #n1 #n2 G ::=
+  Lemma binop_ok_plus_int_int (n1 n2 : Z) G :
+    binop_ok PlusOp #n1 #n2 G :-
       return G #(n1 + n2).
   Proof. Admitted.
-  Definition check_binop_plus_int_int_inst := [instance check_binop_plus_int_int].
-  Global Existing Instance check_binop_plus_int_int_inst.
-  Lemma check_binop_minus_int_int (n1 n2 : Z) G :
-    check_binop MinusOp #n1 #n2 G ::=
+  Definition binop_ok_plus_int_int_inst := [instance binop_ok_plus_int_int].
+  Global Existing Instance binop_ok_plus_int_int_inst.
+  Lemma binop_ok_minus_int_int (n1 n2 : Z) G :
+    binop_ok MinusOp #n1 #n2 G :-
       return G #(n1 - n2).
   Proof. Admitted.
-  Definition check_binop_minus_int_int_inst := [instance check_binop_minus_int_int].
-  Global Existing Instance check_binop_minus_int_int_inst.
+  Definition binop_ok_minus_int_int_inst := [instance binop_ok_minus_int_int].
+  Global Existing Instance binop_ok_minus_int_int_inst.
 
   Lemma main_code_correct :
     ⊢ [{
-      _ ← {check_expr main_code};
+      _ ← {expr_ok main_code};
       done
     }].
   Proof.
@@ -149,25 +188,25 @@ Section proofs.
     repeat liTStep; liShow.
   Abort.
 
-  Lemma check_expr_assert e G :
-    check_expr (Assert e) G ::=
-      v ← {check_expr e};
-      exhale (⌜v = #true⌝);
+  Lemma expr_ok_assert e G :
+    expr_ok (Assert e) G :-
+      v ← {expr_ok e};
+      exhale ⌜v = #true⌝;
       return G #0.
   Proof. Admitted.
-  Definition check_expr_assert_inst := [instance check_expr_assert].
-  Global Existing Instance check_expr_assert_inst.
+  Definition expr_ok_assert_inst := [instance expr_ok_assert].
+  Global Existing Instance expr_ok_assert_inst.
 
-  Lemma check_binop_eq_int_int (n1 n2 : Z) G :
-    check_binop EqOp #n1 #n2 G ::=
+  Lemma binop_ok_eq_int_int (n1 n2 : Z) G :
+    binop_ok EqOp #n1 #n2 G :-
       return G #(bool_decide (n1 = n2)).
   Proof. Admitted.
-  Definition check_binop_eq_int_int_inst := [instance check_binop_eq_int_int].
-  Global Existing Instance check_binop_eq_int_int_inst.
+  Definition binop_ok_eq_int_int_inst := [instance binop_ok_eq_int_int].
+  Global Existing Instance binop_ok_eq_int_int_inst.
 
   Lemma main_code_correct :
     ⊢ [{
-      _ ← {check_expr main_code};
+      _ ← {expr_ok main_code};
       done
     }].
   Proof.
@@ -183,13 +222,14 @@ Section proofs.
   Admitted.
 
   Lemma prove_fn_spec X a e pre post :
-    fn_spec (LamV a e) X pre post ::=
+    fn_spec (LamV a e) X pre post :-
       ∀ (x : X) v,
       inhale pre x v;
-      v' ← {check_expr (subst' a v e)};
+      v' ← {expr_ok (subst' a v e)};
       exhale post x v';
       done.
-  Proof. Admitted.
+  Proof.
+  Admitted.
 
   Lemma add_one_correct :
     ⊢ fn_spec add_one_code Z (λ n v, ⌜v = #n⌝) (λ n v, ⌜v = #(n + 1)⌝).
@@ -207,7 +247,7 @@ Section proofs.
   Lemma main_param_code_correct add_one :
     ⊢ [{
       inhale fn_spec add_one Z (λ n v, ⌜v = #n⌝) (λ n v, ⌜v = #(n + 1)⌝);
-      _ ← {check_expr (main_param_code add_one)};
+      _ ← {expr_ok (main_param_code add_one)};
       done
     }].
   Proof.
@@ -215,25 +255,29 @@ Section proofs.
     repeat liTStep; liShow.
   Abort.
 
-  Lemma check_expr_App e1 e2 G :
-    check_expr (App e1 e2) G ::=
-      v2 ← {check_expr e2};
-      v1 ← {check_expr e1};
+  Lemma expr_ok_App e1 e2 G :
+    (* TODO: have where `{!TCIsNotVal e1} syntax to add typeclass preconditions *)
+    expr_ok (App e1 e2) G  :-
+      v2 ← {expr_ok e2};
+      v1 ← {expr_ok e1};
+     (* TODO: can one have a better notation that does not duplicate
+     the pattern? *)
       '(existT X (pre, post)) ←
-        {find_in_context (FindDirect (λ '(existT X (pre, post)), fn_spec v1 X pre post))};
+        {find_in_context (FindDirect
+             (λ '(existT X (pre, post)), fn_spec v1 X pre post))};
       ∃ x,
       exhale (pre x v2);
       ∀ v',
       inhale (post x v');
       return G v'.
   Proof. Admitted.
-  Definition check_expr_App_inst := [instance check_expr_App].
-  Global Existing Instance check_expr_App_inst | 50.
+  Definition expr_ok_App_inst := [instance expr_ok_App].
+  Global Existing Instance expr_ok_App_inst | 50.
 
   Lemma main_param_code_correct add_one :
     ⊢ [{
       inhale fn_spec add_one Z (λ n v, ⌜v = #n⌝) (λ n v, ⌜v = #(n + 1)⌝);
-      _ ← {check_expr (main_param_code add_one)};
+      _ ← {expr_ok (main_param_code add_one)};
       done
     }].
   Proof.
@@ -251,11 +295,11 @@ Section proofs.
          "f" ("x" - #1) + "f" ("x" - #2).
 
   Lemma prove_fn_spec_rec X f a e pre post :
-    fn_spec (RecV f a e) X pre post ::=
+    fn_spec (RecV f a e) X pre post :-
       ∀ (x : X) v vr,
       inhale pre x v;
       inhale fn_spec vr X pre post;
-      v' ← {check_expr (subst' a v (subst' f vr e))};
+      v' ← {expr_ok (subst' a v (subst' f vr e))};
       exhale post x v';
       done.
   Proof. Admitted.
@@ -269,34 +313,36 @@ Section proofs.
   Abort.
 
 
-  Lemma check_expr_if e0 e1 e2 G :
-    check_expr (If e0 e1 e2) G ::=
-      v ← {check_expr e0};
-      {check_if v (check_expr e1 G) (check_expr e2 G)}.
+  Lemma expr_ok_if e0 e1 e2 G :
+    expr_ok (If e0 e1 e2) G :-
+      v ← {expr_ok e0};
+      {if_ok v (expr_ok e1 G) (expr_ok e2 G)}.
   Proof. Admitted.
-  Definition check_expr_if_inst := [instance check_expr_if].
-  Global Existing Instance check_expr_if_inst.
+  Definition expr_ok_if_inst := [instance expr_ok_if].
+  Global Existing Instance expr_ok_if_inst.
 
-  Lemma check_if_0 G1 G2 :
-    check_if #0 G1 G2 ::= return G2.
+  Lemma if_ok_0 G1 G2 :
+    (* TODO: This is a good usecase for using Typeclass preconditions
+    (i.e. showing whether the boolean is provable).*)
+    if_ok #0 G1 G2 :- return G2.
   Proof. Admitted.
-  Definition check_if_0_inst := [instance check_if_0].
-  Global Existing Instance check_if_0_inst | 2.
+  Definition if_ok_0_inst := [instance if_ok_0].
+  Global Existing Instance if_ok_0_inst | 2.
 
-  Lemma check_if_1 G1 G2 :
-    check_if #1 G1 G2 ::= return G1.
+  Lemma if_ok_1 G1 G2 :
+    if_ok #1 G1 G2 :- return G1.
   Proof. Admitted.
-  Definition check_if_1_inst := [instance check_if_1].
-  Global Existing Instance check_if_1_inst | 2.
+  Definition if_ok_1_inst := [instance if_ok_1].
+  Global Existing Instance if_ok_1_inst | 2.
 
-  Lemma check_if_bool (b : bool) G1 G2 :
-    check_if #b G1 G2 ::=
+  Lemma if_ok_bool (b : bool) G1 G2 :
+    if_ok #b G1 G2 :-
       and:
       | inhale ⌜b⌝; return G1
       | inhale ⌜¬ b⌝; return G2.
   Proof. Admitted.
-  Definition check_if_bool_inst := [instance check_if_bool].
-  Global Existing Instance check_if_bool_inst | 10.
+  Definition if_ok_bool_inst := [instance if_ok_bool].
+  Global Existing Instance if_ok_bool_inst | 10.
 
   Lemma fib_correct :
     ⊢ fn_spec fib_code unit (λ _ v, ∃ n : Z, ⌜v = #n⌝ ∗ ⌜0 ≤ n⌝)
@@ -358,7 +404,7 @@ Section proofs.
   Abort.
 
   Lemma simplify_goal_is_list_null xs G :
-    simplify_goal (is_list #NULL xs) G ::= exhale ⌜xs = []⌝; return G.
+    simplify_goal (is_list #NULL xs) G :- exhale ⌜xs = []⌝; return G.
   Proof. Admitted.
   Definition simplify_goal_is_list_null_inst := [instance simplify_goal_is_list_null with 50%N].
   Global Existing Instance simplify_goal_is_list_null_inst.
@@ -380,40 +426,40 @@ Section proofs.
     repeat liTStep; liShow.
   Abort.
 
-  Lemma check_expr_unop op e G :
-    check_expr (UnOp op e) G ::=
-      v ← {check_expr e};
-      vr  ← {check_unop op v};
+  Lemma expr_ok_unop op e G :
+    expr_ok (UnOp op e) G :-
+      v ← {expr_ok e};
+      vr  ← {unop_ok op v};
       return G vr.
   Proof. Admitted.
-  Definition check_expr_unop_inst := [instance check_expr_unop].
-  Global Existing Instance check_expr_unop_inst.
+  Definition expr_ok_unop_inst := [instance expr_ok_unop].
+  Global Existing Instance expr_ok_unop_inst.
 
-  Lemma check_unop_fst v1 v2 G :
-    check_unop FstOp (v1, v2) G ::= return G v1.
+  Lemma unop_ok_fst v1 v2 G :
+    unop_ok FstOp (v1, v2) G :- return G v1.
   Proof. Admitted.
-  Definition check_unop_fst_inst := [instance check_unop_fst].
-  Global Existing Instance check_unop_fst_inst.
-  Lemma check_unop_snd v1 v2 G :
-    check_unop SndOp (v1, v2) G ::= return G v2.
+  Definition unop_ok_fst_inst := [instance unop_ok_fst].
+  Global Existing Instance unop_ok_fst_inst.
+  Lemma unop_ok_snd v1 v2 G :
+    unop_ok SndOp (v1, v2) G :- return G v2.
   Proof. Admitted.
-  Definition check_unop_snd_inst := [instance check_unop_snd].
-  Global Existing Instance check_unop_snd_inst.
+  Definition unop_ok_snd_inst := [instance unop_ok_snd].
+  Global Existing Instance unop_ok_snd_inst.
 
-  Lemma check_binop_pair v1 v2 G :
-    check_binop PairOp v1 v2 G ::= return G (v1, v2)%V.
+  Lemma binop_ok_pair v1 v2 G :
+    binop_ok PairOp v1 v2 G :- return G (v1, v2)%V.
   Proof. Admitted.
-  Definition check_binop_pair_inst := [instance check_binop_pair].
-  Global Existing Instance check_binop_pair_inst.
+  Definition binop_ok_pair_inst := [instance binop_ok_pair].
+  Global Existing Instance binop_ok_pair_inst.
 
-  Lemma check_expr_alloc G :
-    check_expr Alloc G ::=
+  Lemma expr_ok_alloc G :
+    expr_ok Alloc G :-
       ∀ l : loc,
       inhale (l ↦ #0);
       return G #l.
   Proof. Admitted.
-  Definition check_expr_alloc_inst := [instance check_expr_alloc].
-  Global Existing Instance check_expr_alloc_inst.
+  Definition expr_ok_alloc_inst := [instance expr_ok_alloc].
+  Global Existing Instance expr_ok_alloc_inst.
 
   Lemma cons_correct :
     ⊢ fn_spec cons_code (val * list val)
@@ -428,26 +474,26 @@ Section proofs.
   {| fic_A := (loc * val); fic_Prop '(l, vr) := (⌜v = #l⌝ ∗ l ↦ vr)%I; |}.
   Global Typeclasses Opaque FindMapsTo.
 
-  Lemma check_expr_store e1 e2 G :
-    check_expr (Store e1 e2) G ::=
-      v2 ← {check_expr e2};
-      v1 ← {check_expr e1};
+  Lemma expr_ok_store e1 e2 G :
+    expr_ok (Store e1 e2) G :-
+      v2 ← {expr_ok e2};
+      v1 ← {expr_ok e1};
       '(l, _) ← {find_in_context (FindMapsTo v1)};
       inhale (l ↦ v2);
       return G v2.
   Proof. Admitted.
-  Definition check_expr_store_inst := [instance check_expr_store].
-  Global Existing Instance check_expr_store_inst.
+  Definition expr_ok_store_inst := [instance expr_ok_store].
+  Global Existing Instance expr_ok_store_inst.
 
-  Lemma check_expr_load e G :
-    check_expr (Load e) G ::=
-      v ← {check_expr e};
+  Lemma expr_ok_load e G :
+    expr_ok (Load e) G :-
+      v ← {expr_ok e};
       '(l, vl) ← {find_in_context (FindMapsTo v)};
       inhale (l ↦ vl);
       return G vl.
   Proof. Admitted.
-  Definition check_expr_load_inst := [instance check_expr_load].
-  Global Existing Instance check_expr_load_inst.
+  Definition expr_ok_load_inst := [instance expr_ok_load].
+  Global Existing Instance expr_ok_load_inst.
 
   Lemma cons_correct :
     ⊢ fn_spec cons_code (val * list val)
@@ -458,8 +504,16 @@ Section proofs.
     repeat liTStep; liShow.
   Abort.
 
+  (* TODO : find in context should probably use a different syntax
+     such that it is clear that this is not a usual existential
+     quantifier and exhale. Maybe something like the following? *)
+  (*
+    find_in_context (FindMapsTo #l) G :-
+      pattern: 'v, l ↦ v;
+      return G (l, v).
+  *)
   Lemma find_in_context_find_mapsto_loc (l : loc) G:
-    find_in_context (FindMapsTo #l) G ::=
+    find_in_context (FindMapsTo #l) G :-
       ∃ v,
       exhale (l ↦ v);
       return G (l, v).
@@ -481,7 +535,7 @@ Section proofs.
   {| fic_A := iProp Σ; fic_Prop P := P; |}.
   Global Typeclasses Opaque FindList.
   Lemma find_in_context_find_list_loc (l : loc) G:
-    find_in_context (FindList #l) G ::=
+    find_in_context (FindList #l) G :-
       ∃ v, exhale l ↦ v; return G (l ↦ v).
   Proof. iDestruct 1 as (v) "[Hl HT]". iExists _. by iFrame. Qed.
   Definition find_in_context_find_list_loc_inst :=
@@ -500,7 +554,7 @@ Section proofs.
   Abort.
 
   Lemma subsume_mapsto_list (l : loc) v xs G :
-    subsume (l ↦ v) (is_list #l xs) G ::=
+    subsume (l ↦ v) (is_list #l xs) G :-
      ∃ v1 v2 xs',
      exhale ⌜v = (v1, v2)%V⌝ ∗ ⌜xs = v2 :: xs'⌝ ∗ is_list v1 xs';
      return G.
@@ -527,7 +581,7 @@ Section proofs.
   Abort.
 
   Lemma find_in_context_find_list_list v G:
-    find_in_context (FindList v) G ::=
+    find_in_context (FindList v) G :-
       ∃ xs, exhale is_list v xs; return G (is_list v xs).
   Proof. iDestruct 1 as (xs) "[Hl HT]". iExists _. by iFrame. Qed.
   Definition find_in_context_find_list_list_inst :=
@@ -535,7 +589,7 @@ Section proofs.
   Global Existing Instance find_in_context_find_list_list_inst | 1.
 
   Lemma subsume_list_list v xs1 xs2 G :
-    subsume (is_list v xs1) (is_list v xs2) G ::=
+    subsume (is_list v xs1) (is_list v xs2) G :-
      exhale ⌜xs1 = xs2⌝;
      return G.
   Proof. Admitted.
@@ -565,8 +619,9 @@ Section proofs.
   Abort.
 
   Lemma find_in_context_find_mapsto_list v G:
-    find_in_context (FindMapsTo v) G ::=
+    find_in_context (FindMapsTo v) G :-
       ∃ xs, exhale is_list v xs;
+
       exhale ⌜0 < length xs⌝;
       ∀ (l : loc) v' x xs',
       inhale ⌜v = #l⌝ ∗ ⌜xs = x::xs'⌝ ∗ is_list v' xs';
@@ -612,13 +667,13 @@ Section proofs.
       match o with | Some l => ⌜v = #l⌝ | None => ⌜v = #NULL⌝ end%I : iProp Σ; |}.
   Global Typeclasses Opaque FindLocOrNULL.
 
-  Lemma check_binop_eq_val_NULL v G :
-    check_binop EqOp v #NULL G ::=
+  Lemma binop_ok_eq_val_NULL v G :
+    binop_ok EqOp v #NULL G :-
       o ← {find_in_context (FindLocOrNULL v)};
       return G #(if o is Some _ then false else true).
   Proof. Admitted.
-  Definition check_binop_eq_val_NULL_inst := [instance check_binop_eq_val_NULL].
-  Global Existing Instance check_binop_eq_val_NULL_inst.
+  Definition binop_ok_eq_val_NULL_inst := [instance binop_ok_eq_val_NULL].
+  Global Existing Instance binop_ok_eq_val_NULL_inst.
 
   Lemma length_correct :
     ⊢ fn_spec length_code (val * list val)
@@ -630,7 +685,7 @@ Section proofs.
   Abort.
 
   Lemma find_in_context_find_locornull_list v G:
-    find_in_context (FindLocOrNULL v) G ::=
+    find_in_context (FindLocOrNULL v) G :-
       ∃ xs, exhale is_list v xs;
       and:
       | inhale ⌜xs = []⌝ ∗ ⌜v = #NULL⌝; return G None
